dimsum/iris/iris.v
@@ -1,4 +1,4 @@
 From dimsum.core Require Export module trefines.
-From dimsum.core.iris Require Export sat sim expr spec combinators.
+From dimsum.core.iris Require Export sat sim combinators.
 
 (** This file reexports all relevant modules and should be imported by clients. *)
