dimsum/iris/spec2.v
@@ -1,0 +1,322 @@
+From dimsum.core Require Export spec_mod.
+From dimsum.core.iris Require Export sim expr2.
+Set Default Proof Using "Type".
+
+Definition spec_state_interp {Σ EV S} (state_interp : S → iProp Σ) : (spec EV S void * S) → option S → iProp Σ :=
+  λ s os, if os is Some s' then ⌜s.2 = s'⌝%I else state_interp s.2.
+
+Arguments spec_state_interp _ _ _ _ _ !_ /.
+
+Program Definition spec_mod_lang {Σ} (EV S : Type) (state_interp : S → iProp Σ)  : mod_lang EV Σ := {|
+  mexpr := spec EV S void;
+  mectx := unit;
+  mstate := S;
+  mfill _ := id;
+  mcomp_ectx _ _:= tt;
+  mtrans := spec_trans EV S;
+  mexpr_rel σ t := σ.1 ≡ t;
+  mstate_interp := spec_state_interp state_interp;
+|}.
+Next Obligation. done. Qed.
+
+Definition spec_mod_lang_unit {Σ} (EV : Type) : mod_lang EV Σ :=
+  spec_mod_lang EV unit (λ _, True%I).
+
+Section spec.
+  Context `{!dimsumGS Σ} {EV S : Type} {state_interp : S → iProp Σ}.
+
+  Global Instance sim_gen_expr_spec_proper ts J :
+    Proper ((≡) ==> (=) ==> (=) ==> (⊣⊢)) (sim_gen_expr (Λ:=spec_mod_lang EV S state_interp) ts J).
+  Proof.
+    move => ?? ? ?? -> ?? ->.
+    rewrite !sim_gen_expr_unfold /sim_gen_expr_pre/=. by repeat f_equiv.
+  Qed.
+
+  Let X := (spec_mod_lang EV _ state_interp).
+  Local Canonical Structure X.
+
+  Lemma sim_gen_TVis ts k J Φ e os :
+    (∀ s, ▷ₒ?ts imodhandle (S:=m_state (spec_trans _ _)) J (Some e) (k tt, s) (λ σ', spec_state_interp state_interp σ' os ∗ WP{ts} σ'.1 @ ? os, J {{ Φ }})) -∗
+    WP{ts} (Spec.bind (TVis e) k) @ ? os, J {{ Φ }}.
+  Proof.
+    iIntros "Hsim". rewrite unfold_bind/=. setoid_rewrite unfold_bind; simpl.
+  Admitted.
+    (* iApply sim_tgt_expr_step. iIntros (?[??]?? Heq Hstep) "Hs". simplify_eq/=. iModIntro. *)
+    (* inv/= Hstep. *)
+    (* all: revert select (_ ≡ _); rewrite {1}Heq; try by move => /spec_equiv_inv. *)
+    (* move => /spec_equiv_inv //= [? Heq2]. simplify_eq/=. *)
+    (* iSplit!. iIntros "Htgt". iApply "Hsim". by iApply "Htgt". *)
+  (* Qed. *)
+
+  (* Lemma sim_src_TVis k J Φ e os : *)
+  (*   ▷ₒ imodhandle J (Some e) (SRC k tt @ ? os, J {{ Φ }}) -∗ *)
+  (*   SRC (Spec.bind (TVis e) k) @ ? os, J {{ Φ }}. *)
+  (* Proof. *)
+  (*   iIntros "Hsim". rewrite unfold_bind/=. setoid_rewrite unfold_bind; simpl. *)
+  (* Admitted. *)
+  (*   iApply sim_src_expr_step. iIntros (?[??]?) "?". simplify_eq/=. iModIntro. *)
+  (*   iExists _, _. iSplit. { iPureIntro. by econs. } *)
+  (*   iIntros ([??] ?) "!> HΦ". simplify_eq. *)
+  (*   iApply "Hsim". iIntros (?) "?". by iApply ("HΦ" with "[//] [$]"). *)
+  (* Qed. *)
+
+  (* TODO: This is missing lemmas for going from @ ? None to @ ? Some and back. *)
+  Lemma sim_gen_TGet ts k J Φ s :
+    (▷ₒ?ts WP{ts} (k s) @ s, J {{ Φ }}) -∗
+    WP{ts} (Spec.bind TGet k) @ s, J {{ Φ }}.
+  Proof.
+    iIntros "Hsim". rewrite unfold_bind/=. setoid_rewrite unfold_bind; simpl.
+  Admitted.
+  (*   iApply sim_tgt_expr_step_None. iIntros (?[??]?? Heq Hstep ?). simplify_eq/=. iModIntro. *)
+  (*   inv/= Hstep. *)
+  (*   all: revert select (_ ≡ _); rewrite {1}Heq; try by move => /spec_equiv_inv. *)
+  (*   move => /spec_equiv_inv //= Heq2. simplify_eq/=. *)
+  (*   iSplit!. iModIntro. rewrite Heq2. iSplit!. by iFrame. *)
+  (* Qed. *)
+
+  (* Lemma sim_src_TGet k Π Φ s : *)
+  (*   SRC (k s) @ s [{ Π }] {{ Φ }} -∗ *)
+  (*   SRC (Spec.bind TGet k) @ s [{ Π }] {{ Φ }}. *)
+  (* Proof. *)
+  (*   iIntros "Hsim". rewrite unfold_bind/=. setoid_rewrite unfold_bind; simpl. *)
+  (*   iApply sim_src_expr_step_None. iIntros (?[??]? ?). simplify_eq/=. iModIntro. *)
+  (*   iExists _. iSplit. { iPureIntro. by econs. } *)
+  (*   iIntros ([??] ?) "!>". simplify_eq. iSplit!. by iFrame. *)
+  (* Qed. *)
+
+  Lemma sim_gen_TPut ts k J Φ s s' :
+    (▷ₒ?ts WP{ts} (k tt) @ s', J {{ Φ }}) -∗
+    WP{ts} (Spec.bind (TPut s') k) @ s, J {{ Φ }}.
+  Proof.
+    iIntros "Hsim". rewrite unfold_bind/=. setoid_rewrite unfold_bind; simpl.
+  Admitted.
+  (*   iApply sim_tgt_expr_step_None. iIntros (?[??]?? Heq Hstep ?). simplify_eq/=. iModIntro. *)
+  (*   inv/= Hstep. *)
+  (*   all: revert select (_ ≡ _); rewrite {1}Heq; try by move => /spec_equiv_inv. *)
+  (*   move => /spec_equiv_inv //= [? Heq2]. simplify_eq/=. *)
+  (*   iSplit!. iModIntro. rewrite Heq2. iSplit!. by iFrame. *)
+  (* Qed. *)
+
+  (* Lemma sim_src_TPut k Π Φ s s' : *)
+  (*   SRC (k tt) @ s' [{ Π }] {{ Φ }} -∗ *)
+  (*   SRC (Spec.bind (TPut s') k) @ s [{ Π }] {{ Φ }}. *)
+  (* Proof. *)
+  (*   iIntros "Hsim". rewrite unfold_bind/=. setoid_rewrite unfold_bind; simpl. *)
+  (*   iApply sim_src_expr_step_None. iIntros (?[??]? ?). simplify_eq/=. iModIntro. *)
+  (*   iExists _. iSplit. { iPureIntro. by econs. } *)
+  (*   iIntros ([??] ?) "!>". simplify_eq. iSplit!. by iFrame. *)
+  (* Qed. *)
+
+  Lemma sim_gen_TAll {T} ts k J Φ os :
+    (∃/∀{ts} x, ▷ₒ?ts WP{ts} (k x) @ ? os, J {{ Φ }}) -∗
+    WP{ts} (Spec.bind (TAll T) k) @ ? os, J {{ Φ }}.
+  Proof.
+    iIntros "Hsim". rewrite unfold_bind/=. setoid_rewrite unfold_bind; simpl.
+  Admitted.
+
+  Lemma sim_tgt_TAll {T} x k J Φ os :
+    (▷ₒ TGT (k x) @ ? os, J {{ Φ }}) -∗
+    TGT (Spec.bind (TAll T) k) @ ? os, J {{ Φ }}.
+  Proof. iIntros "Hsim". iApply sim_gen_TAll => /=. by iExists _. Qed.
+  Lemma sim_src_TAll {T} k J Φ os :
+    (∀ x, SRC (k x) @ ? os, J {{ Φ }}) -∗
+    SRC (Spec.bind (TAll T) k) @ ? os, J {{ Φ }}.
+  Proof. iIntros "Hsim". by iApply sim_gen_TAll => /=. Qed.
+
+  (* Lemma sim_src_TAll {T} k Π Φ os : *)
+  (*   (∀ x, SRC (k x) @ ? os [{ Π }] {{ Φ }}) -∗ *)
+  (*   SRC (Spec.bind (TAll T) k) @ ? os [{ Π }] {{ Φ }}. *)
+  (* Proof. *)
+  (*   iIntros "Hsim". rewrite unfold_bind/=. setoid_rewrite unfold_bind; simpl. *)
+  (*   iApply sim_src_expr_step_None. iIntros (?[??]?) "?". simplify_eq/=. iModIntro. *)
+  (*   iExists _. iSplit. { iPureIntro. by econs. } *)
+  (*   iIntros ([??] [??]) "!>". simplify_eq. iSplit!. iFrame. iApply "Hsim". *)
+  (* Qed. *)
+
+  Lemma sim_gen_TExist {T} ts k J Φ os :
+    (∀/∃{ts} x, ▷ₒ?ts WP{ts} (k x) @ ? os, J {{ Φ }}) -∗
+    WP{ts} (Spec.bind (TExist T) k) @ ? os, J {{ Φ }}.
+  Proof.
+    iIntros "Hsim". rewrite unfold_bind/=. setoid_rewrite unfold_bind; simpl.
+  Admitted.
+
+  Lemma sim_tgt_TExist {T} k J Φ os :
+    (∀ x, ▷ₒ TGT (k x) @ ? os, J {{ Φ }}) -∗
+    TGT (Spec.bind (TExist T) k) @ ? os, J {{ Φ }}.
+  Proof. iIntros "Hsim". by iApply sim_gen_TExist => /=. Qed.
+  Lemma sim_src_TExist {T} x k J Φ os :
+    (SRC (k x) @ ? os, J {{ Φ }}) -∗
+    SRC (Spec.bind (TExist T) k) @ ? os, J {{ Φ }}.
+  Proof. iIntros "Hsim". iApply sim_gen_TExist => /=. by iExists _. Qed.
+
+  (* Lemma sim_tgt_TExist {T} k Π Φ os : *)
+  (*   (∀ x, ▷ₒ TGT (k x) @ ? os [{ Π }] {{ Φ }}) -∗ *)
+  (*   TGT (Spec.bind (TExist T) k) @ ? os [{ Π }] {{ Φ }}. *)
+  (* Proof. *)
+  (*   iIntros "Hsim". rewrite unfold_bind/=. setoid_rewrite unfold_bind; simpl. *)
+  (*   iApply sim_tgt_expr_step_None. iIntros (?[??]?? Heq Hstep) "Hs". simplify_eq/=. iModIntro. *)
+  (*   inv/= Hstep. *)
+  (*   all: revert select (_ ≡ _); rewrite {1}Heq; try by move => /spec_equiv_inv. *)
+  (*   move => /spec_equiv_inv //= [? Heq2]. simplify_eq/=. iSpecialize ("Hsim" $! _). *)
+  (*   iSplit!. iModIntro. rewrite Heq2. iSplit!. iFrame. *)
+  (* Qed. *)
+
+  (* Lemma sim_src_TExist {T} x k Π Φ os : *)
+  (*   SRC (k x) @ ? os [{ Π }] {{ Φ }} -∗ *)
+  (*   SRC (Spec.bind (TExist T) k) @ ? os [{ Π }] {{ Φ }}. *)
+  (* Proof. *)
+  (*   iIntros "Hsim". rewrite unfold_bind/=. setoid_rewrite unfold_bind; simpl. *)
+  (*   iApply sim_src_expr_step_None. iIntros (?[??]?) "?". simplify_eq/=. iModIntro. *)
+  (*   iExists _. iSplit. { iPureIntro. by econs. } *)
+  (*   iIntros ([??] ?) "!>". simplify_eq. iSplit!. iFrame. *)
+  (* Qed. *)
+
+  (* TODO: Can these proofs be derived from the proofs before? *)
+  Lemma sim_tgt_TNb T (k : T → _) J Φ os :
+    ⊢ TGT (Spec.bind TNb k) @ ? os , J {{ Φ }}.
+  Proof.
+    rewrite unfold_bind/=. setoid_rewrite unfold_bind; simpl.
+  Admitted.
+    (* iApply sim_tgt_expr_step_None. iIntros (?[??]?? Heq Hstep) "Hs". simplify_eq/=. iModIntro. *)
+    (* inv/= Hstep. *)
+    (* all: revert select (_ ≡ _); rewrite {1}Heq; try by move => /spec_equiv_inv. *)
+    (* move => /spec_equiv_inv //= [? Heq2]. simplify_eq/=. destruct_all void. *)
+  (* Qed. *)
+
+  Lemma sim_tgt_TNb_end J Φ os :
+    ⊢ TGT TNb @ ? os, J {{ Φ }}.
+  Proof.
+  Admitted.
+    (* iApply sim_tgt_expr_step_None. iIntros (?[??]?? Heq Hstep) "Hs". simplify_eq/=. iModIntro. *)
+    (* inv/= Hstep. *)
+    (* all: revert select (_ ≡ _); rewrite {1}Heq; try by move => /spec_equiv_inv. *)
+    (* move => /spec_equiv_inv //= [? Heq2]. simplify_eq/=. destruct_all void. *)
+  (* Qed. *)
+
+  Lemma sim_src_TUb T (k : T → _) J Φ os :
+    ⊢ SRC (Spec.bind TUb k) @ ? os, J {{ Φ }}.
+  Proof.
+  Admitted.
+    (* rewrite unfold_bind/=. setoid_rewrite unfold_bind; simpl. *)
+    (* iApply sim_src_expr_step_None. iIntros (?[??]?) "?". simplify_eq/=. iModIntro. *)
+    (* iExists _. iSplit. { iPureIntro. by econs. } *)
+    (* iIntros ([??] [??]) "!>". destruct_all void. *)
+  (* Qed. *)
+
+  Lemma sim_src_TUb_end J Φ os :
+    ⊢ SRC TUb @ ? os, J {{ Φ }}.
+  Proof.
+  Admitted.
+    (* iApply sim_src_expr_step_None. iIntros (?[??]?) "?". simplify_eq/=. iModIntro. *)
+    (* iExists _. iSplit. { iPureIntro. by econs. } *)
+    (* iIntros ([??] [??]) "!>". destruct_all void. *)
+  (* Qed. *)
+
+  Lemma sim_gen_TAssume ts k J Φ (P : Prop) os :
+    (⌜P⌝ ∗/-∗{ts} ▷ₒ?ts WP{ts} (k tt) @ ? os, J {{ Φ }}) -∗
+    WP{ts} (Spec.bind (TAssume P) k) @ ? os, J {{ Φ }}.
+  Proof.
+    iIntros "Hsim". rewrite unfold_bind/=. setoid_rewrite unfold_bind; simpl.
+  Admitted.
+
+  Lemma sim_tgt_TAssume k J Φ (P : Prop) os :
+    P →
+    (▷ₒ TGT (k tt) @ ? os, J {{ Φ }}) -∗
+    TGT (Spec.bind (TAssume P) k) @ ? os, J {{ Φ }}.
+  Proof. iIntros (?) "?". iApply sim_gen_TAssume. by iFrame. Qed.
+  Lemma sim_src_TAssume k J Φ (P : Prop) os :
+    (⌜P⌝ -∗ SRC (k tt) @ ? os, J {{ Φ }}) -∗
+    SRC (Spec.bind (TAssume P) k) @ ? os, J {{ Φ }}.
+  Proof. iIntros "?". by iApply sim_gen_TAssume. Qed.
+  (*   iIntros (?) "Hsim". rewrite unfold_bind/=. setoid_rewrite unfold_bind; simpl. *)
+  (*   iApply sim_tgt_expr_step_None. iIntros (?[??]?? Heq Hstep) "Hs". simplify_eq/=. iModIntro. *)
+  (*   inv/= Hstep. *)
+  (*   all: revert select (_ ≡ _); rewrite {1}Heq; try by move => /spec_equiv_inv. *)
+  (*   move => /spec_equiv_inv //= [? Heq2]. simplify_eq/=. *)
+  (*   iSplit!. iModIntro. rewrite Heq2. iSplit!. iFrame. *)
+  (*   Unshelve. done. *)
+  (* Qed. *)
+
+  (* Lemma sim_src_TAssume k Π Φ P os : *)
+  (*   (⌜P⌝ -∗ SRC (k tt) @ ? os [{ Π }] {{ Φ }}) -∗ *)
+  (*   SRC (Spec.bind (TAssume P) k) @ ? os [{ Π }] {{ Φ }}. *)
+  (* Proof. *)
+  (*   iIntros "Hsim". rewrite unfold_bind/=. setoid_rewrite unfold_bind; simpl. *)
+  (*   iApply sim_src_expr_step_None. iIntros (?[??]?) "?". simplify_eq/=. iModIntro. *)
+  (*   iExists _. iSplit. { iPureIntro. by econs. } *)
+  (*   iIntros ([??] [??]) "!>". simplify_eq. iSplit!. iFrame. by iApply "Hsim". *)
+  (* Qed. *)
+
+  Lemma sim_gen_TAssert ts k J Φ (P : Prop) os :
+    (⌜P⌝ -∗/∗{ts} ▷ₒ?ts WP{ts} (k tt) @ ? os, J {{ Φ }}) -∗
+    WP{ts} (Spec.bind (TAssert P) k) @ ? os, J {{ Φ }}.
+  Proof.
+    iIntros "Hsim". rewrite unfold_bind/=. setoid_rewrite unfold_bind; simpl.
+  Admitted.
+
+  Lemma sim_tgt_TAssert k J Φ (P : Prop) os :
+    (⌜P⌝ -∗ ▷ₒ TGT (k tt) @ ? os, J {{ Φ }}) -∗
+    TGT (Spec.bind (TAssert P) k) @ ? os, J {{ Φ }}.
+  Proof. iIntros "?". by iApply sim_gen_TAssert. Qed.
+  Lemma sim_src_TAssert k J Φ (P : Prop) os :
+    P →
+    (SRC (k tt) @ ? os, J {{ Φ }}) -∗
+    SRC (Spec.bind (TAssert P) k) @ ? os, J {{ Φ }}.
+  Proof. iIntros (?) "?". iApply sim_gen_TAssert. by iFrame. Qed.
+
+  (* Lemma sim_tgt_TAssert k Π Φ (P : Prop) os : *)
+  (*   (⌜P⌝ -∗ ▷ₒ TGT (k tt) @ ? os [{ Π }] {{ Φ }}) -∗ *)
+  (*   TGT (Spec.bind (TAssert P) k) @ ? os [{ Π }] {{ Φ }}. *)
+  (* Proof. *)
+  (*   iIntros "Hsim". rewrite unfold_bind/=. setoid_rewrite unfold_bind; simpl. *)
+  (*   iApply sim_tgt_expr_step_None. iIntros (?[??]?? Heq Hstep) "Hs". simplify_eq/=. iModIntro. *)
+  (*   inv/= Hstep. *)
+  (*   all: revert select (_ ≡ _); rewrite {1}Heq; try by move => /spec_equiv_inv. *)
+  (*   move => /spec_equiv_inv //= [? Heq2]. simplify_eq/=. iSpecialize ("Hsim" with "[//]"). *)
+  (*   iSplit!. iModIntro. rewrite Heq2. iSplit!. iFrame. *)
+  (* Qed. *)
+
+  (* Lemma sim_src_TAssert k Π Φ (P : Prop) os : *)
+  (*   P → *)
+  (*   SRC (k tt) @ ? os [{ Π }] {{ Φ }} -∗ *)
+  (*   SRC (Spec.bind (TAssert P) k) @ ? os [{ Π }] {{ Φ }}. *)
+  (* Proof. *)
+  (*   iIntros (?) "Hsim". rewrite unfold_bind/=. setoid_rewrite unfold_bind; simpl. *)
+  (*   iApply sim_src_expr_step_None. iIntros (?[??]?) "?". simplify_eq/=. iModIntro. *)
+  (*   iExists _. iSplit. { iPureIntro. by econs. } *)
+  (*   iIntros ([??] ?) "!>". simplify_eq. iSplit!. iFrame. *)
+  (*   Unshelve. done. *)
+  (* Qed. *)
+
+  Lemma sim_tgt_TAssumeOpt {T} o (x : T) k J Φ os :
+    o = Some x →
+    TGT k x @ ? os , J {{ Φ }} -∗
+    TGT (Spec.bind (TAssumeOpt o) k) @ ? os , J {{ Φ }}.
+  Proof. iIntros (->) "Hsim". simpl. by rewrite unfold_bind/=. Qed.
+
+  Lemma sim_src_TAssumeOpt {T} (o : option T) k J Φ os :
+    (∀ x, ⌜o = Some x⌝ -∗ SRC k x @ ? os, J {{ Φ }}) -∗
+    SRC (Spec.bind (TAssumeOpt o) k) @ ? os, J {{ Φ }}.
+  Proof.
+    iIntros "Hsim".
+    destruct o => /=.
+    - rewrite unfold_bind/=. by iApply "Hsim".
+    - iApply sim_src_TUb.
+  Qed.
+
+  Lemma sim_tgt_TAssertOpt {T} (o : option T) k J Φ os :
+    (∀ x, ⌜o = Some x⌝ -∗ TGT k x @ ? os, J {{ Φ }}) -∗
+    TGT (Spec.bind (TAssertOpt o) k) @ ? os, J {{ Φ }}.
+  Proof.
+    iIntros "Hsim".
+    destruct o => /=.
+    - rewrite unfold_bind/=. by iApply "Hsim".
+    - iApply sim_tgt_TNb.
+  Qed.
+
+  Lemma sim_src_TAssertOpt {T} o (x : T) k J Φ os :
+    o = Some x →
+    SRC k x @ ? os, J {{ Φ }} -∗
+    SRC (Spec.bind (TAssertOpt o) k) @ ? os, J {{ Φ }}.
+  Proof. iIntros (->) "Hsim". simpl. by rewrite unfold_bind/=. Qed.
+End spec.
